Generalize FStar.MRef over data invariants
Silence some warnings

ulib/FStar.MRef.fst
@@ -3,26 +3,27 @@ open FStar.Heap
 open FStar.ST
 
 open FStar.Preorder
+open FStar.DataInvariant
 
 let stable (#a:Type) (p:(a -> Type)) (b:preorder a) = forall x y. p x /\ b x y ==> p y
 
-private let p_pred (#a:Type) (#b:preorder a) (r:mref a b) (p:(a -> Type))
+private let p_pred (#a:Type) (#inv:data_inv a) (#rel:preorder a) (r:mref a inv rel) (p:(a -> Type))
   = fun h -> h `contains` r /\ p (sel h r)
 
-abstract let token (#a:Type) (#b:preorder a) (r:mref a b) (p:(a -> Type){stable p b})
+abstract let token (#a:Type) (#inv:data_inv a) (#rel:preorder a) (r:mref a inv rel) (p:(a -> Type){stable p rel})
   = witnessed (p_pred r p)
 
-abstract val take_token: #a:Type -> #b:preorder a -> m:mref a b -> p:(a -> Type){stable p b}
+abstract val take_token: #a:Type -> #inv:data_inv a -> #rel:preorder a -> m:mref a inv rel -> p:(a -> Type){stable p rel}
                          -> ST unit (requires (fun h0 -> p (sel h0 m)))
                                    (ensures (fun h0 _ h1 -> h0==h1 /\ token m p))
-let take_token #a #b m p =
+let take_token #a #inv #rel m p =
   gst_recall (contains_pred m);
   gst_witness (p_pred m p)
 
-abstract val recall_token: #a:Type -> #b:preorder a -> m:mref a b -> p:(a -> Type){stable p b}
+abstract val recall_token: #a:Type -> #inv:data_inv a -> #rel:preorder a -> m:mref a inv rel -> p:(a -> Type){stable p rel}
                            -> ST unit (requires (fun _ ->  token m p))
                                      (ensures (fun h0 _ h1 -> h0==h1 /\ p (sel h1 m)))
-let recall_token #a #b m p = gst_recall (p_pred m p)
+let recall_token #a #inv #rel m p = gst_recall (p_pred m p)
 
 abstract val recall: p:(heap -> Type){ST.stable p}
                      -> ST unit (requires (fun _ ->  witnessed p))
